\begin{cases}
  x_1 & +   x_2  & +   x_3 & +   x_4 & = 2   \\
  x_1 & + 2 x_2  & + 3 x_3 & - 4 x_4 & = 2   \\
2 x_1 & + 3 x_2  & + 5 x_3 & + 9 x_4 & = 2   \\
  x_1 & +   x_2  & + 2 x_3 & + 7 x_4 & = 2   \\
\end{cases} \\

D = \begin{vmatrix}
1 &  1 & 1 &  1  \\ 
1 &  2 & 3 & -4  \\
2 &  3 & 5 &  9  \\
1 &  1 & 2 &  7  \\
\end{vmatrix}
= -6 \not = 0 \\

D_1 = \begin{vmatrix}
2 &  1 & 1 &  1  \\ 
2 &  2 & 3 & -4  \\
2 &  3 & 5 &  9  \\
2 &  1 & 2 &  7  \\
\end{vmatrix}
= -36,


D_2 = \begin{vmatrix}
1 &  2 & 1 &  1  \\ 
1 &  2 & 3 & -4  \\
2 &  2 & 5 &  9  \\
1 &  2 & 2 &  7  \\
\end{vmatrix} =  34 \\

D_3 = \begin{vmatrix}
1 &  1 & 2 &  1  \\ 
1 &  2 & 2 & -4  \\
2 &  3 & 2 &  9  \\
1 &  1 & 2 &  7  \\
\end{vmatrix} = -12 ,


D_4 = \begin{vmatrix}
1 &  1 & 1 & 2  \\ 
1 &  2 & 3 & 2  \\
2 &  3 & 5 & 2  \\
1 &  1 & 2 & 2  \\
\end{vmatrix} = 2 \\

x_{1} = \frac{D_{1}}{D} = \frac{-36}{-6} = 6;
x_{2} = \frac{D_{2}}{D} = \frac{34}{-6} = -\frac{17}{3}; \\
x_{3} = \frac{D_{3}}{D} = \frac{-12}{-6} = 2;
x_{4} = \frac{D_{4}}{D} = \frac{2}{-6} = -\frac{1}{3};
