\begin{cases}
3 x_1 & +3 x_2 & -  x_3 & +5 x_4 &=& 0  \\
2 x_1 & -  x_2 & +2 x_3 & -7 x_4 &=& 0  \\
4 x_1 & +  x_2 & -3 x_3 & +6 x_4 &=& 0  \\
  x_1 & -2 x_2 & +4 x_3 & -7 x_4 &=& 0  \\
\end{cases} \\

\begin{pmatrix}
3  &  3   & -1 &  5 \\ 
2  & -1   &  2 & -7 \\
4  &  1   & -3 &  6 \\
1  & -2   &  4 & -7 \\
\end{pmatrix} \xrightarrow[]{(1) \sim (4)}
\begin{pmatrix}
1  & -2   &  4 & -7 \\
2  & -1   &  2 & -7 \\
4  &  1   & -3 &  6 \\
3  &  3   & -1 &  5 \\ 
\end{pmatrix} \\

\xrightarrow[\substack{ (3):=(3)-4(1) \\ (4):=(4)-3(1)  }]{(2):=(2)-2(1)}
\begin{pmatrix}
1  & -2   &  4 & -7  \\
0  &  3   & -6 &  7  \\
0  &  9   &-19 &  34 \\
0  &  9   &-13 &  26 \\
\end{pmatrix} \\
\xrightarrow[(4):=(4)-3(2)]{(3):=(3)-3(2)}
\begin{pmatrix}
1  & -2   &  4 & -7  \\
0  &  3   & -6 &  7  \\
0  &  0   & -1 & 13  \\
0  &  0   &  5 &  5  \\
\end{pmatrix} \\
\xrightarrow[]{(4):=(4)+5(3)}
\begin{pmatrix}
1  & -2   &  4 & -7  \\
0  &  3   & -6 &  7  \\
0  &  0   & -1 & 13  \\
0  &  0   &  0 & 38  \\
\end{pmatrix}
